working simp tactic with global tags for dist equiv

src/computational_monads/distribution_semantics/tactics/pairwise_dist_equiv.lean
@@ -4,6 +4,7 @@ Released under Apache 2.0 license as described in the file LICENSE.
 Authors: Devon Tuma
 -/
 import computational_monads.distribution_semantics.tactics.by_dist_equiv
+import computational_monads.distribution_semantics.tactics.tactic_tags
 
 /-!
 # Induction Tactic for Splitting an Equivalence into Line by Line Equivalences
@@ -15,22 +16,6 @@ This file defines a tactic `pairwise_dist_equiv` for working with and proving in
 open interactive interactive.types
 
 variables {α β γ : Type} {spec : oracle_spec}
-
-/-- Tag for lemmas to be automatically applied by `pairwise_dist_equiv`. -/
-meta def simp_dist_equiv : user_attribute :=
-{ name := "simp_dist_equiv",
-  descr := "Lemmas tagged with this attribute are automatically called by the
-              `pairwise_dist_equiv` tactic, similar to the way the `simp` tactic works." }
-
-run_cmd attribute.register "simp_dist_equiv"
-
-meta def get_simp_dist_equiv_lemmas : tactic (list pexpr) :=
-do {tagged_d_eqs ← (attribute.get_instances "simp_dist_equiv"),
-  t' ← mmap tactic.get_decl tagged_d_eqs,
-  d ←  return (list.map declaration.value t'),
-  q ← return (list.map pexpr.of_expr d),
-  return q
-}
 
 namespace oracle_comp
 
