src/computational_monads/decidable.lean
@@ -12,7 +12,7 @@ This file defines a typeclass `oracle_comp.decidable` for computations that have
 instances for every return value in the computation.
 We don't currently make use of this in general, becuase `open_locale classical` makes
 it unnecessary, but if this eventually gets removed then things like `oracle_comp.fin_support`
-will require it to function
+will require it to function.
 -/
 
 namespace oracle_comp
