src/computational_monads/distribution_semantics/tactics/tactic_tags.lean
@@ -1,0 +1,32 @@
+/-
+Copyright (c) 2023 Devon Tuma. All rights reserved.
+Released under Apache 2.0 license as described in the file LICENSE.
+Authors: Devon Tuma
+-/
+
+/-!
+# Tags for Marking Distributional Equivalence Lemmas
+
+This file defines a tactic `pairwise_dist_equiv` for working with and proving instances of
+`dist_equiv` between sequenced computations, by splitting the goal into line-by-line equivalences.
+
+TODO: some things in `return` and `bind` files I think.
+-/
+
+open interactive interactive.types
+
+/-- Tag for lemmas to be automatically applied by `pairwise_dist_equiv`. -/
+meta def simp_dist_equiv : user_attribute :=
+{ name := "simp_dist_equiv",
+  descr := "Lemmas tagged with this attribute are automatically called by the
+              `pairwise_dist_equiv` tactic, similar to the way the `simp` tactic works." }
+
+run_cmd attribute.register "simp_dist_equiv"
+
+meta def get_simp_dist_equiv_lemmas : tactic (list pexpr) :=
+do {tagged_d_eqs ← (attribute.get_instances "simp_dist_equiv"),
+  t' ← mmap tactic.get_decl tagged_d_eqs,
+  d ←  return (list.map declaration.value t'),
+  q ← return (list.map pexpr.of_expr d),
+  return q
+}
